---
title: Lista1
author: Pedro Correa
output: pdf_document
---

4. Prove por definição as seguintes afirmações:

a. $n^{2} = O(n^{3})$

> $$ n^{2} \le c*n^{3} $$
>
> $$ 1 \le c*n $$
>
> $c = 1$ | $n > 1$

b. $2*n^{2} + 1 = O(n^{2})$

> $$ 2*n^{2} + 1 \le c*n^{2} $$
>
> $$ 2*n^{2} - c*n^{2} \le -1 $$
>
> $$ n^{2}*(2 - c) \le -1 $$
>
> $c > 2$ | $n > 0$

c. $n^{2} + 3*n + 7 = \Omega(6*n + 7)$

> $$ n^{2} + 3*n + 7 \ge c*(6*n + 7) $$
>
> $$ n^{2} + 3*n + 7 \ge 6*c*n + 7*c $$
>
> $$ n^{2} + 3*n - 6*c*n - 7*c \ge -7 $$
>
> $$ n(n + 3 - 6*c) - 7*c \ge -7 $$
>
> $$c = \frac{1}{2}; n \ge 2$$

d. $1000 * n = o(\frac{n^{2}}{1000})$

> $$ 1000 * n < c*(\frac{n^{2}}{1000}) $$
>
> $$ 1000 < \frac{c * n}{1000} $$
>
> $$ 1000 * 1000 < c * n $$
>
> $$ 10^{6} < c * n $$
>
> $$ \frac{10^{6}}{c} < n $$

e. $\frac{1}{2} * n * ( n + 1 ) = \Theta(n^{2})$

> $$c1 * n^{2} \le \frac{1}{2} * n * ( n + 1 )$$
>
> $$c1 * n^{2} \le \frac{1}{2} * n^{2} + \frac{1}{2} * n$$
>
> $$c1 * n \le \frac{1}{2} * n + \frac{1}{2}$$
>
> $$c1 * n - \frac{1}{2} * n \le \frac{1}{2}$$
>
> $$c1 = \frac{1}{4}; n = 1$$


> $$\frac{1}{2} * n * ( n + 1 ) \le c2 * n^{2}$$
>
> $$\frac{1}{2} * n^{2} + \frac{1}{2} * n \le c2 * n^{2}$$
>
> $$\frac{1}{2} * n + \frac{1}{2} \le c2 * n$$
>
> $$\frac{1}{2} \le c2 * n - \frac{1}{2} * n$$
>
> $$c2 = 1; n > 1$$

f. $\log^{2}(n) = \Omega(\log(n^{2}))$

> $$\log^{2}(n) \ge c * \log(n^{2})$$
>
> $$\log(n) * \log(n) \ge 2 * c * \log(n)$$
>
> $$\log(n) \ge 2 * c$$
>
> $c = 1$ | $n \ge 4$

g. $10 * n^{2} + 12 * n + 6 = \Theta(2 * n^{2} - n)$

> $$10 * n^{2} + 12 * n + 6 \le c1 * (2 * n^{2} - n)$$
>
> $$10 * n^{2} + 12 * n + 6 \le 2 * c1 * n^{2} - c1 * n$$
>
> $$10 * n^{2} - 2 * c1 * n^{2} + 12 * n + c1 * n \le - 6$$
>
> $$n * (10 * n - 2 * c1 * n + 12 + c1) \le - 6$$

> $$c1 * (2 * n^{2} - n) \le 10 * n^{2} + 12 * n + 6$$
>
> $$ 2 * c1 * n^{2} - c1 * n \le 10 * n^{2} + 12 * n + 6$$
>
> $$-6 \le 10 * n^{2} - 2 * c1 * n^{2} + 12 * n + c1 * n$$
>
> $$-6 \le n * (10 * n - 2 * c1 * n + 12 + c1)$$

h. $2^{n + 1} = O(2^{n})$

> $$2^{n + 1} \le c * (2^{n})$$
>
> $$\frac{2^{n + 1}}{2^{n}} \le c$$
>
> $$2^{n + 1 - n} \le c$$
>
> $$2 \le c$$

i. $2^{2 * n} = O(2^{n})$

> $$2^{2 * n} \le c * 2^{n}$$
>
> $$2^{n} * 2^{n} \le c * 2^{n}$$
>
> $$2^{n} \le c$$
>
> $$c = 1$$
